Thread eta expansion everywhere (#676)
* Thread eta-expandedness assumptions through all the compilation passes

* Prove preservation of eta expanded fixpoints through erasure

* WIP fixing remaining eta-expansion glitches

* We need to eta-expand constructors as well to get preservation by let-expansion

* Produce properly eta-expanded contexts in inductive declarations

* Eta expansion preservation in PCUIC

* Show that Template to PCUIC preserve eta-expanded environments

* Refactor the various transformations so they live in their right place in Template/PCUIC/Erasure

* Refactor Erasure into multiple files, defining the structures, transfomations and the final pipeline

* Disable eta-expansion for now as it seems to produce ill-typed terms

* Add a template program that allows

* Add a metacoq program that allows to test well-typedness of expanded quoted programs.
This could be run systematically to perform translation-validation of the eta-expansion phase, but would be quite costly.

* Comment debug printing which can have very large output

* Fix build problem

* Fix safechecker

template-coq/src/constr_denoter.ml
@@ -113,6 +113,8 @@ struct
       Constr.DEFAULTcast
     else if constr_equall trm kNative then
       Constr.VMcast
+    else if constr_equall trm kRevertCast then
+      Constr.REVERTcast
     else
       not_supported_verb trm "unquote_cast_kind"
 
@@ -366,6 +368,7 @@ struct
   : (Constr.t, quoted_int, quoted_ident, quoted_name, quoted_sort, quoted_cast_kind, quoted_kernel_name, 
     quoted_inductive, quoted_relevance, quoted_univ_instance, quoted_proj, 
     quoted_int63, quoted_float64) structure_of_term =
+    (* debug (fun () -> Pp.(str "denote_term" ++ spc () ++ print_term t)) ; *)
     let (h,args) = app_full t [] in
     if constr_equall h tRel then
       match args with
