template-coq/src/denoter.ml
@@ -64,7 +64,7 @@ struct
   let denote_term (env : Environ.env) (evm : Evd.evar_map) (trm: D.t) : Evd.evar_map * Constr.t =
     let open Context.Rel.Declaration in
     let rec aux env evm (trm: D.t) : _ * Constr.t =
-      (*    debug (fun () -> Pp.(str "denote_term" ++ spc () ++ pr_constr trm)) ; *)
+      (* debug (fun () -> Pp.(str "denote_term" ++ spc () ++ Printer.pr_econstr_env env evm trm)) ;  *)
       match D.inspect_term trm with
       | ACoq_tRel x -> evm, Constr.mkRel (D.unquote_int x + 1)
       | ACoq_tVar x -> evm, Constr.mkVar (D.unquote_ident x)
