erasure/theories/Erasure.v
@@ -1,437 +1,75 @@
 (* Distributed under the terms of the MIT license. *)
 From Coq Require Import Program ssreflect ssrbool.
-From MetaCoq.Template Require Import config utils uGraph Pretty Environment Typing WcbvEval.
-Set Warnings "-notation-overridden".
-From MetaCoq.PCUIC Require Import PCUICAst PCUICAstUtils PCUICTyping
-     TemplateToPCUIC TemplateToPCUICCorrectness TemplateToPCUICWcbvEval.
-From MetaCoq.PCUIC Require PCUICExpandLets PCUICExpandLetsCorrectness.
-Set Warnings "+notation-overridden".
-From MetaCoq.SafeChecker Require Import PCUICErrors PCUICWfEnvImpl.
-From MetaCoq.Erasure Require Import EAstUtils ErasureFunction ErasureCorrectness EPretty Extract.
-From MetaCoq.Erasure Require ErasureFunction EOptimizePropDiscr ERemoveParams EWcbvEval EDeps.
+From MetaCoq.Template Require Import Transform bytestring config utils.
+From MetaCoq.PCUIC Require PCUICAst PCUICAstUtils PCUICProgram.
+From MetaCoq.Erasure Require EAstUtils ErasureFunction ErasureCorrectness EPretty Extract.
+From MetaCoq.Erasure Require Import ETransform.
 
-#[local] Instance extraction_checker_flags : checker_flags := 
-  {| check_univs := true;
-     prop_sub_type := false;
-     indices_matter := false;
-     lets_in_constructor_types := true |}.
+Import PCUICProgram.
+Import TemplateProgram (template_eta_expand).
+Import PCUICTransform (template_to_pcuic_transform, pcuic_expand_lets_transform).
 
-(* Used to show timings of the ML execution *)
- 
-Definition time : forall {A B}, string -> (A -> B) -> A -> B :=
-  fun A B s f x => f x.
-
-Extract Constant time => 
-  "(fun c f x -> let s = Caml_bytestring.caml_string_of_bytestring c in Tm_util.time (Pp.str s) f x)".
+Import bytestring.
+Local Open Scope bs.
+Local Open Scope string_scope2.
 
 (* This is the total erasure function +
   let-expansion of constructor arguments and case branches +
   shrinking of the global environment dependencies +
   the optimization that removes all pattern-matches on propositions. *)
 
-Import EOptimizePropDiscr.
-
-Module Transform.
-  Section Opt.
-     Context {program program' : Type}.
-     Context {value value' : Type}.
-     Context {eval :  program -> value -> Type}.
-     Context {eval' : program' -> value' -> Type}.
-     
-     Definition preserves_eval pre (transform : forall p : program, pre p -> program') obseq :=
-      forall p v (pr : pre p),
-        eval p v ->
-        let p' := transform p pr in
-        exists v',
-        ∥ eval' p' v' × obseq p p' v v' ∥.
-
-    Record t := 
-    { name : string; 
-      pre : program -> Prop; 
-      transform : forall p : program, pre p -> program';
-      post : program' -> Prop;
-      correctness : forall input (p : pre input), post (transform input p);
-      obseq : program -> program' -> value -> value' -> Prop;
-      preservation : preserves_eval pre transform obseq; }.
-
-    Definition run (x : t) (p : program) (pr : pre x p) : program' := 
-      time x.(name) (fun _ => x.(transform) p pr) tt.
-
-  End Opt.
-  Arguments t : clear implicits.
-
-  Section Comp.
-    Context {program program' program'' : Type}.
-    Context {value value' value'' : Type}.
-    Context {eval : program -> value -> Type}.
-    Context {eval' : program' -> value' -> Type}.
-    Context {eval'' : program'' -> value'' -> Type}.
-    
-    Obligation Tactic := idtac.
-    Program Definition compose (o : t program program' value value' eval eval') (o' : t program' program'' value' value'' eval' eval'') 
-      (hpp : (forall p, o.(post) p -> o'.(pre) p)) : t program program'' value value'' eval eval'' :=
-      {| 
-        name := o.(name) ^ " -> " ^ o'.(name);
-        transform p hp := run o' (run o p hp) (hpp _ (o.(correctness) _ hp));
-        pre := o.(pre);
-        post := o'.(post);
-        obseq g g' v v' := exists g'' v'', o.(obseq) g g'' v v'' × o'.(obseq) g'' g' v'' v'
-        |}.
-    Next Obligation.
-      intros o o' hpp inp pre.
-      eapply o'.(correctness).
-    Qed.
-    Next Obligation.
-      red. intros o o' hpp.
-      intros p v pr ev.
-      eapply o.(preservation) in ev; auto.
-      cbn in ev. destruct ev as [v' [ev]].
-      epose proof (o'.(preservation) (o.(transform) p pr) v').
-      specialize (H (hpp _ (o.(correctness) _ pr))).
-      destruct ev. specialize (H e).
-      destruct H as [v'' [[ev' obs']]].
-      exists v''. constructor. split => //.
-      exists (transform o p pr), v'. now split.
-    Qed.
-  End Comp.
-End Transform.
-
 Import Transform.
-Obligation Tactic := idtac.
-
-Definition self_transform program value eval eval' := Transform.t program program value value eval eval'.
-
-Definition pcuic_program := 
-  global_env_ext_map * term.
-
-Definition eval_program (p : Ast.Env.program) (v : Ast.term) :=
-  WcbvEval.eval p.1 p.2 v.  
-  
-Definition eval_pcuic_program (p : pcuic_program) (v : term) :=
-  PCUICWcbvEval.eval p.1.(trans_env_env) p.2 v.
-
-Definition template_to_pcuic_obseq (p : Ast.Env.program) (p' : pcuic_program) (v : Ast.term) (v' : term) :=
-  let Σ := Ast.Env.empty_ext p.1 in v' = trans (trans_global Σ) v.
-  
-Program Definition template_to_pcuic_transform {cf : checker_flags} : 
-  Transform.t Ast.Env.program pcuic_program Ast.term term 
-  eval_program eval_pcuic_program :=
- {| name := "template to pcuic";
-    pre p :=  
-      let Σ := Ast.Env.empty_ext p.1 in
-      ∥ Typing.wf_ext Σ × ∑ T, Typing.typing (Ast.Env.empty_ext p.1) [] p.2 T ∥;
-    transform p hp := let Σ' := trans_global (Ast.Env.empty_ext p.1) in 
-      (Σ', trans Σ' p.2) ;
-    post p := ∥ wf_ext p.1 × ∑ T, typing p.1 [] p.2 T ∥;
-    obseq := template_to_pcuic_obseq |}.
-Next Obligation.
-  intros cf [Σ t] [[wfext ht]].
-  set (Σ' := trans_global _).
-  cbn. sq. split => //. eapply template_to_pcuic_env_ext. apply wfext.
-  destruct ht as [T HT]. exists (trans (trans_global_env Σ) T).
-  eapply (template_to_pcuic_typing (Σ := Ast.Env.empty_ext Σ) []). apply wfext.
-  apply HT.
-Qed.
-Next Obligation.
-  red. intros cf [Σ t] v [[]].
-  unfold eval_pcuic_program, eval_program.
-  cbn. intros ev.
-  unshelve eapply TemplateToPCUICWcbvEval.trans_wcbvEval in ev; eauto. apply w.
-  eexists; split; split; eauto. red. reflexivity.
-  eapply template_to_pcuic_env.
-  apply w. destruct s as [T HT]. apply TypingWf.typing_wf in HT. apply HT. auto.
-Qed.
-
-Program Definition build_global_env_map (g : global_env) : global_env_map := 
-  {| trans_env_env := g; 
-     trans_env_map := EnvMap.EnvMap.of_global_env g.(declarations) |}.
-Next Obligation.
-  intros g. eapply EnvMap.EnvMap.repr_global_env.
-Qed.
-
-Import EGlobalEnv.
-
-Definition eprogram := 
-  (EAst.global_context * EAst.term).
-
-Import EEnvMap.GlobalContextMap (make, global_decls).
-
-Arguments EWcbvEval.eval {wfl} _ _ _.
-
-Definition eval_eprogram (wfl : EWcbvEval.WcbvFlags) (p : eprogram) (t : EAst.term) := 
-  EWcbvEval.eval (wfl:=wfl) p.1 p.2 t.
-
-Program Definition optimize_prop_discr_optimization : self_transform eprogram EAst.term (eval_eprogram EWcbvEval.default_wcbv_flags) (eval_eprogram EWcbvEval.opt_wcbv_flags) := 
-  {| name := "optimize_prop_discr"; 
-    transform p _ := 
-      (EOptimizePropDiscr.optimize_env p.1, EOptimizePropDiscr.optimize p.1 p.2);
-    pre p := (closed_env p.1 /\ ELiftSubst.closedn 0 p.2);
-    post p := (closed_env p.1 /\ ELiftSubst.closedn 0 p.2);
-    obseq g g' v v' := v' = EOptimizePropDiscr.optimize g.1 v
-    |}.
-
-Next Obligation.
-  intros [Σ t] [cle clt].
-  cbn in *. split.
-  move: cle. induction Σ at 1 3; cbn; auto.
-  move/andP => [] cla clg. rewrite (IHg clg) andb_true_r.
-  destruct a as [kn []]; cbn in * => //.
-  destruct E.cst_body => //. cbn in cla |- *.
-  now eapply EOptimizePropDiscr.closed_optimize.
-  now eapply EOptimizePropDiscr.closed_optimize.
-Qed.
-Next Obligation.
-  red. move=> [Σ t] /= v [cle clt] ev.
-  eapply EOptimizePropDiscr.optimize_correct in ev; eauto.
-Qed.
-
-Lemma wf_glob_fresh Σ : wf_glob Σ -> EnvMap.EnvMap.fresh_globals Σ.
-Proof.
-  induction Σ. constructor; auto.
-  intros wf; depelim wf. constructor; auto.
-Qed.
-
-Definition eprogram_env := 
-  (EEnvMap.GlobalContextMap.t * EAst.term).
-
-Definition eval_eprogram_env (wfl : EWcbvEval.WcbvFlags) (p : eprogram_env) (t : EAst.term) := 
-  EWcbvEval.eval (wfl:=wfl) p.1.(global_decls) p.2 t.
-
-Program Definition remove_params (p : eprogram_env) : eprogram :=
-  (ERemoveParams.strip_env p.1, ERemoveParams.strip p.1 p.2).
-
-Program Definition remove_params_optimization (fl : EWcbvEval.WcbvFlags) : 
-  Transform.t eprogram_env eprogram EAst.term EAst.term (eval_eprogram_env fl) (eval_eprogram fl) :=
-  {| name := "remove_parameters";
-    transform p pre := remove_params p;
-    pre p := 
-    let decls := p.1.(global_decls) in
-     [/\ wf_glob decls, EEtaExpanded.isEtaExp_env decls, 
-      EEtaExpanded.isEtaExp decls p.2, closed_env decls & ELiftSubst.closedn 0 p.2];
-    post p := (closed_env p.1 /\ ELiftSubst.closedn 0 p.2);
-    obseq g g' v v' := v' = (ERemoveParams.strip g.1 v) |}.
-Next Obligation.
-  intros fl [Σ t] [wfe etae etat cle clt].
-  simpl.
-  cbn -[ERemoveParams.strip] in *.
-  split.
-  move: cle. unfold closed_env. unfold ERemoveParams.strip_env.
-  rewrite forallb_map. eapply forallb_impl. intros.
-  destruct x as [kn []]; cbn in * => //.
-  destruct E.cst_body => //. cbn -[ERemoveParams.strip] in H0 |- *.
-  now eapply ERemoveParams.closed_strip.
-  now eapply ERemoveParams.closed_strip.
-Qed.
-Next Obligation.
-  red. move=> ? [Σ t] /= v [wfe etae etat cle clt] ev.
-  eapply ERemoveParams.strip_eval in ev; eauto. 
-Qed.
-
-Program Definition remove_params_fast_optimization (fl : EWcbvEval.WcbvFlags) :
-  Transform.t eprogram_env eprogram EAst.term EAst.term (eval_eprogram_env fl) (eval_eprogram fl) :=
-  {| name := "remove_parameters_fast";
-    transform p _ := (ERemoveParams.Fast.strip_env p.1, ERemoveParams.Fast.strip p.1 [] p.2);
-    pre p := 
-      let decls := p.1.(global_decls) in
-      [/\ wf_glob decls, EEtaExpanded.isEtaExp_env decls, 
-       EEtaExpanded.isEtaExp decls p.2, closed_env decls & ELiftSubst.closedn 0 p.2];
-    post p := (closed_env p.1 /\ ELiftSubst.closedn 0 p.2);
-    obseq g g' v v' := v' = (ERemoveParams.strip g.1 v) |}.
-Next Obligation.
-  intros fl [Σ t] [wfe etae etat cle clt].
-  simpl.
-  rewrite -ERemoveParams.Fast.strip_fast -ERemoveParams.Fast.strip_env_fast.
-  cbn -[ERemoveParams.strip] in *.
-  split.
-  move: cle. unfold closed_env. unfold ERemoveParams.strip_env.
-  rewrite forallb_map. eapply forallb_impl. intros.
-  destruct x as [kn []]; cbn in * => //.
-  destruct E.cst_body => //. cbn -[ERemoveParams.strip] in H0 |- *.
-  now eapply ERemoveParams.closed_strip.
-  now eapply ERemoveParams.closed_strip.
-Qed.
-Next Obligation.
-  red. move=> ? [Σ t] /= v [wfe etae etat cle clt] ev.
-  rewrite -ERemoveParams.Fast.strip_fast -ERemoveParams.Fast.strip_env_fast.
-  eapply ERemoveParams.strip_eval in ev; eauto.
-Qed.
-
-
-Definition let_expansion_obseq (p : pcuic_program) (p' : pcuic_program) (v : term) (v' : term) :=
-  v' = PCUICExpandLets.trans v.
-
-Program Definition pcuic_expand_lets_transform {cf : checker_flags} : 
-  self_transform pcuic_program term eval_pcuic_program eval_pcuic_program :=
- {| name := "let expansion in branches/constructors";
-    pre p :=
-      let Σ : global_env_ext := p.1 in
-      ∥ wf_ext Σ × ∑ T, typing Σ nil p.2 T ∥;
-    transform p hp := 
-      let Σ' := PCUICExpandLets.trans_global p.1 in 
-      ((build_global_env_map Σ', p.1.2), PCUICExpandLets.trans p.2) ;
-    post p := ∥ wf_ext (H:=PCUICExpandLetsCorrectness.cf' cf) p.1 × 
-      ∑ T, typing (H:=PCUICExpandLetsCorrectness.cf' cf) p.1 nil p.2 T ∥;
-    obseq := let_expansion_obseq |}.
-Next Obligation.
-  intros cf [Σ t] [[wfext ht]].
-  set (Σ' := PCUICExpandLets.trans_global _).
-  cbn. sq. unfold build_global_env_map. unfold global_env_ext_map_global_env_ext. simpl.
-  split. eapply PCUICExpandLetsCorrectness.trans_wf_ext in wfext. apply wfext.
-  destruct ht as [T HT]. exists (PCUICExpandLets.trans T).
-  eapply (PCUICExpandLetsCorrectness.pcuic_expand_lets Σ []) => //.
-  apply wfext. apply PCUICExpandLetsCorrectness.trans_wf_ext in wfext. apply wfext.
-Qed.
-Next Obligation.
-  red. intros cf [Σ t] v [[]].
-  unfold eval_pcuic_program.
-  cbn. intros ev.
-  unshelve eapply (PCUICExpandLetsCorrectness.trans_wcbveval (Σ:=Σ)) in ev; eauto.
-  eexists; split; split; eauto. red. reflexivity.
-  destruct s as [T HT]. now apply PCUICClosedTyp.subject_closed in HT.
-Qed.
 
 Obligation Tactic := program_simpl.
 
-Definition build_wf_env_from_env {cf : checker_flags} (Σ : global_env_map) (wfΣ : ∥ wf Σ ∥) : wf_env := 
-  {| wf_env_referenced := {| referenced_impl_env := Σ.(trans_env_env); referenced_impl_wf := wfΣ |} ;
-     wf_env_map := Σ.(trans_env_map);
-     wf_env_map_repr := Σ.(trans_env_repr);
- |}.
+#[local] Existing Instance extraction_checker_flags.
 
-Program Definition erase_pcuic_program (p : pcuic_program) 
-  (wfΣ : ∥ wf_ext (H := config.extraction_checker_flags) p.1 ∥)
-  (wt : ∥ ∑ T, typing (H := config.extraction_checker_flags) p.1 [] p.2 T ∥) : eprogram_env :=
-  let wfe := build_wf_env_from_env p.1.1 (map_squash (wf_ext_wf _) wfΣ) in
-  let wfe' := make_wf_env_ext wfe p.1.2 wfΣ in
-  let t := ErasureFunction.erase wfe' nil p.2 _ in
-  let Σ' := ErasureFunction.erase_global (term_global_deps t) wfe in
-  (EEnvMap.GlobalContextMap.make Σ' _, t).
-  
-Next Obligation.
-  sq. destruct wt as [T Ht].
-  cbn in *. subst. now exists T.
-Qed.
-Next Obligation.
-  unfold erase_global.
-  eapply wf_glob_fresh.
-  eapply ERemoveParams.erase_global_decls_wf_glob.
-Qed.
+Import EWcbvEval.
 
-(* * The full correctness lemma of erasure from Template programs do λ-box
-
-Lemma erase_template_program_correctness {p : Ast.Env.program} univs
-  (Σ := (p.1, univs))
-  {wfΣ : ∥ Typing.wf_ext Σ ∥}
-  {wt : ∥ ∑ T, Typing.typing (p.1, univs) [] p.2 T ∥} {Σ' t'} :
-  erase_template_program p univs wfΣ wt = (Σ', t') ->
-  forall v, WcbvEval.eval p.1 p.2 v ->
-  exists v',
-    PCUICExpandLets.trans_global (trans_global Σ) ;;; [] |- 
-      PCUICExpandLets.trans (trans (trans_global Σ) v) ⇝ℇ v' /\ 
-    ∥ EWcbvEval.eval (wfl:=EWcbvEval.default_wcbv_flags) Σ' t' v' ∥.
-Proof.
-  unfold erase_template_program.
-  intros [= <- <-] v ev.
-  set (expΣ := (PCUICExpandLets.trans_global (trans_global Σ))).
-  set (wfexpΣ := build_wf_env _ _).
-  pose proof (erase_correct wfexpΣ).
-  set (wfexpΣ' := make_wf_env_ext _ _ _) in *.
-  set wftΣ : ∥ wf_ext (PCUICExpandLets.trans_global (trans_global Σ)) ∥ :=
-    wfexpΣ'.(wf_env_ext_wf).
-  specialize (H univs wftΣ (PCUICExpandLets.trans (trans (trans_global Σ) p.2)) (PCUICExpandLets.trans (trans (trans_global Σ) v))).
-  set wtp : PCUICSafeLemmata.welltyped (PCUICExpandLets.trans_global (trans_global Σ)) [] 
-    (PCUICExpandLets.trans (trans (trans_global Σ) p.2)) :=
-    (erase_template_program_obligation_1 p univs wfΣ wt).
-  set (t' := erase wfexpΣ' [] (PCUICExpandLets.trans (trans (trans_global_env p.1) p.2)) wtp) in *.
-  set (deps := (term_global_deps _)).
-  (* change (empty_ext (PCUICExpandLets.trans_global_env (trans_global_env p.1))) with *)
-    (* (PCUICExpandLets.trans_global (trans_global Σ)) in *. *)
-  specialize (H (erase_global deps wfexpΣ)).
-  specialize (H _ deps wtp eq_refl).
-  forward H. eapply Kernames.KernameSet.subset_spec. reflexivity.
-  specialize (H eq_refl).
-  destruct wt, wfΣ.
-  have wfmid : wf (trans_global (p.1, univs)).1.
-  { now eapply template_to_pcuic_env. }
-  forward H.
-  { unfold wfexpΣ. simpl.
-    unshelve eapply (PCUICExpandLetsCorrectness.trans_wcbveval (Σ := (trans_global_env p.1, univs))).
-    { destruct s as [T HT].
-      eapply (PCUICClosedTyp.subject_closed (Γ := [])). 
-      apply (template_to_pcuic_typing (Σ := (p.1, univs)) [] _ T);simpl; eauto.
-      eapply w. Unshelve. now eapply template_to_pcuic_env. }
-    unshelve eapply trans_wcbvEval; eauto. apply w.
-    destruct s as [T HT]. eauto.
-    clear -w HT. now eapply TypingWf.typing_wf in HT. }  
-  destruct H as [v' [Hv He]].
-  sq.
-  set (eΣ := erase_global _ _) in *. exists v'. split => //.
-Qed. *)
-
-Obligation Tactic := idtac.
-
-Program Definition erase_transform : Transform.t pcuic_program eprogram_env term EAst.term eval_pcuic_program (eval_eprogram_env EWcbvEval.default_wcbv_flags) :=
- {| name := "erasure";
-    pre p :=  
-      ∥ wf_ext (H := config.extraction_checker_flags) p.1 × ∑ T, typing (H := config.extraction_checker_flags) p.1 [] p.2 T ∥;
-    transform p hp := erase_pcuic_program p (map_squash fst hp) (map_squash snd hp) ;
-    post p :=
-      let decls := p.1.(global_decls) in
-      [/\ wf_glob decls, closed_env decls & ELiftSubst.closedn 0 p.2];
-    obseq g g' v v' := let Σ := g.1 in Σ ;;; [] |- v ⇝ℇ v' |}.
-Next Obligation.
-  intros [Σ t] [[wfext ht]].
-  destruct erase_pcuic_program eqn:e.
-  unfold erase_pcuic_program in e. simpl. injection e. intros <- <-. split.
-  eapply ERemoveParams.erase_global_wf_glob.
-  eapply erase_global_closed.
-  eapply (erases_closed _ []). 2:eapply erases_erase.
-  clear e. destruct ht as [T HT].
-  now eapply (@PCUICClosedTyp.subject_closed _ _) in HT.
-Qed.
-Next Obligation.
-  red. move=> [Σ t] v [[wf [T HT]]]. unfold eval_pcuic_program, eval_eprogram.
-  intros ev.
-  destruct erase_pcuic_program eqn:e.
-  unfold erase_pcuic_program in e. simpl in e. injection e; intros <- <-.
-  simpl. clear e. cbn in *.
-  set (Σ' := build_wf_env_from_env _ _).
-  (* assert (wt : PCUICSafeLemmata.welltyped (cf:=config.extraction_checker_flags) Σ [] t). now exists T. *)
-  eapply (erase_correct Σ' Σ.2 _ _ _ _ _ (term_global_deps _)) in ev; try reflexivity.
-  2:eapply Kernames.KernameSet.subset_spec; reflexivity.
-  destruct ev as [v' [he [hev]]]. exists v'; split; split => //.
-  red. cbn.
-  eexact hev.
-Qed.
-
-Obligation Tactic := program_simpl.
-
-Local Notation " o ▷ o' " := (Transform.compose o o' _) (at level 50, left associativity).
-
-Program Definition erasure_pipeline := 
+Program Definition erasure_pipeline :
+ Transform.t TemplateProgram.template_program EProgram.eprogram 
+  Ast.term EAst.term
+  TemplateProgram.eval_template_program
+  (EProgram.eval_eprogram {| with_prop_case := false; with_guarded_fix := false |}) := 
+  (* Eta expansion of constructors and fixpoints *)
+  template_eta_expand ▷
+  (* Casts are removed, application is binary, case annotations are inferred from the global environment *)
   template_to_pcuic_transform ▷
+  (* Branches of cases are expanded to bind only variables, constructor types are expanded accordingly *)
   pcuic_expand_lets_transform ▷
-  erase_transform ▷ 
-  remove_params_optimization _ ▷ 
+  (* Erasure of proofs terms in Prop and types *)
+  erase_transform ▷
+  (* Simulation of the guarded fixpoint rules with a single unguarded one: the only "stuck" fixpoints 
+     remaining are unapplied.  *)
+  guarded_to_unguarded_fix eq_refl ▷
+  (* Remove all constructor parameters *)
+  remove_params_optimization ▷ 
+  (* Remove all cases of propositional content *)
   optimize_prop_discr_optimization.
 
 Next Obligation.
-  destruct H. split => //. all:todo "etaexp".
+  destruct H. split => //. sq.
+  now eapply EProgram.expanded_eprogram_expanded_eprogram_cstrs. 
 Qed.
 
-Definition erase_program := run erasure_pipeline.
+(* For now we only give out that erased programs are closed, but 
+  they are also eta-expanded and well-scoped w.r.t. the global environment *)
+Eval simpl in post (guarded_to_unguarded_fix _).
+
+Definition run_erase_program := run erasure_pipeline.
 
 Program Definition erasure_pipeline_fast := 
+  template_eta_expand ▷
   template_to_pcuic_transform ▷
   pcuic_expand_lets_transform ▷
   erase_transform ▷ 
   remove_params_fast_optimization _ ▷ 
   optimize_prop_discr_optimization.
 Next Obligation.
-  destruct H; split => //. all:todo "etaexp".
+  destruct H; split => //. now eapply EProgram.expanded_eprogram_expanded_eprogram_cstrs. 
 Qed.
 
-Definition erase_program_fast := run erasure_pipeline_fast.
+Definition run_erase_program_fast := run erasure_pipeline_fast.
 
 Local Open Scope string_scope.
 
@@ -439,12 +77,12 @@ Local Open Scope string_scope.
   are welltyped (for speed). As such this should only be used for testing, or when we know that 
   the environment is wellformed and the term well-typed (e.g. when it comes directly from a 
   Coq definition). *)
-Program Definition erase_and_print_template_program {cf : checker_flags} (p : Ast.Env.program)
+Definition erase_and_print_template_program {cf : checker_flags} (p : Ast.Env.program)
   : string :=
-  let p' := erase_program p (todo "wf_env and welltyped term") in
-  time "Pretty printing" print_program p'.
+  let p' := run_erase_program p (sq (todo "assuming quoted environment and term are well-typed")) in
+  time "Pretty printing" EPretty.print_program p'.
 
 Program Definition erase_fast_and_print_template_program {cf : checker_flags} (p : Ast.Env.program)
   : string :=
-  let p' := erase_program_fast p (todo "wf_env and welltyped term") in
-  time "pretty-printing" print_program p'.
+  let p' := run_erase_program_fast p (sq (todo "wf_env and welltyped term")) in
+  time "pretty-printing" EPretty.print_program p'.
