pcuic/theories/PCUICEtaExpand.v
@@ -1,4 +1,4 @@
-From MetaCoq.PCUIC Require Import PCUICAst PCUICAstUtils PCUICTyping.
+From MetaCoq.PCUIC Require Import PCUICAst PCUICAstUtils PCUICTyping PCUICProgram TemplateToPCUIC.
 
 Definition isConstruct t :=
    match t with tConstruct _ _ _ => true | _ => false end.
@@ -27,7 +27,12 @@ Inductive expanded (Γ : list nat) : term -> Prop :=
 | expanded_tConst (c : kername) (u : Instance.t) : expanded Γ (tConst c u)
 | expanded_tInd (ind : inductive) (u : Instance.t) : expanded Γ (tInd ind u)
 | expanded_tCase (ci : case_info) (type_info:predicate term)
-        (discr:term) (branches : list (branch term)) : expanded Γ discr -> Forall (fun br => expanded (repeat 0 #|br.(bcontext)| ++ Γ) br.(bbody)) branches -> expanded Γ (tCase ci type_info discr branches)
+        (discr:term) (branches : list (branch term)) : expanded Γ discr -> 
+        Forall (expanded Γ) type_info.(pparams) ->
+        Forall (fun br =>
+          ∥ All_fold (fun Δ d => ForOption (fun b => expanded (repeat 0 #|Δ| ++ repeat 0 #|type_info.(pparams)|) b) d.(decl_body)) br.(bcontext) ∥ /\
+          expanded (repeat 0 #|br.(bcontext)| ++ Γ) br.(bbody)) branches -> 
+        expanded Γ (tCase ci type_info discr branches)
 | expanded_tProj (proj : projection) (t : term) : expanded Γ t -> expanded Γ (tProj proj t)
 | expanded_tFix (mfix : mfixpoint term) (idx : nat) args d : 
   Forall (fun d => let ctx := rev_map (fun  d => 1 + d.(rarg)) mfix in expanded (ctx ++ Γ) d.(dbody)) mfix ->
@@ -44,69 +49,77 @@ Inductive expanded (Γ : list nat) : term -> Prop :=
     expanded Γ (mkApps (tConstruct ind c u) args).
 
 End expanded.
+Derive Signature for expanded.
+
+Definition expanded_context Σ Γ ctx :=
+  ∥ All_fold (fun Δ d => ForOption (expanded Σ (repeat 0 #|Δ| ++ Γ)) d.(decl_body)) ctx ∥.
 
 Lemma expanded_ind :
-forall (Σ : global_env) (P : list nat -> term -> Prop),
-(forall (Γ : list nat) (n m : nat) (args : list term),
- nth_error Γ n = Some m ->
- m <= #|args| -> Forall (expanded Σ Γ) args -> Forall (P Γ) args -> P Γ (mkApps (tRel n) args)) ->
-(forall (Γ : list nat) (id : ident), P Γ (tVar id)) ->
-(forall (Γ : list nat) (ev : nat) (args : list term),
- Forall (expanded Σ Γ) args -> Forall (P Γ) args -> P Γ (tEvar ev args)) ->
-(forall (Γ : list nat) (s : Universe.t), P Γ (tSort s)) ->
-(forall (Γ : list nat) (na : aname) (ty body : term), P Γ (tProd na ty body)) ->
-(forall (Γ : list nat) (na : aname) (ty body : term),
- expanded Σ (0 :: Γ) body -> P (0 :: Γ) body -> P Γ (tLambda na ty body)) ->
-(forall (Γ : list nat) (na : aname) (def def_ty body : term),
- expanded Σ Γ def ->
- P Γ def ->
- expanded Σ (0 :: Γ) body ->
- P (0 :: Γ) body -> P Γ (tLetIn na def def_ty body)) ->
-(forall (Γ : list nat) (f6 : term) (args : list term),
-~ (isConstruct f6 || isFix f6 || isRel f6) ->
- expanded Σ Γ f6 ->
- P Γ f6 -> Forall (expanded Σ Γ) args -> Forall (P Γ) args -> P Γ (mkApps f6 args)) ->
-(forall (Γ : list nat) (c : kername) (u : Instance.t), P Γ (tConst c u)) ->
-(forall (Γ : list nat) (ind : inductive) (u : Instance.t), P Γ (tInd ind u)) ->
-(forall (Γ : list nat) (ci : case_info) (type_info : predicate term)
-   (discr : term) (branches : list (branch term)),
- expanded Σ Γ discr ->
- P Γ discr ->
- Forall
-   (fun br : branch term =>
-	expanded Σ (repeat 0 #|bcontext br| ++ Γ) (bbody br)) branches ->
+  forall (Σ : global_env) (P : list nat -> term -> Prop),
+  (forall (Γ : list nat) (n m : nat) (args : list term),
+  nth_error Γ n = Some m ->
+  m <= #|args| -> Forall (expanded Σ Γ) args -> Forall (P Γ) args -> P Γ (mkApps (tRel n) args)) ->
+  (forall (Γ : list nat) (id : ident), P Γ (tVar id)) ->
+  (forall (Γ : list nat) (ev : nat) (args : list term),
+  Forall (expanded Σ Γ) args -> Forall (P Γ) args -> P Γ (tEvar ev args)) ->
+  (forall (Γ : list nat) (s : Universe.t), P Γ (tSort s)) ->
+  (forall (Γ : list nat) (na : aname) (ty body : term), P Γ (tProd na ty body)) ->
+  (forall (Γ : list nat) (na : aname) (ty body : term),
+  expanded Σ (0 :: Γ) body -> P (0 :: Γ) body -> P Γ (tLambda na ty body)) ->
+  (forall (Γ : list nat) (na : aname) (def def_ty body : term),
+  expanded Σ Γ def ->
+  P Γ def ->
+  expanded Σ (0 :: Γ) body ->
+  P (0 :: Γ) body -> P Γ (tLetIn na def def_ty body)) ->
+  (forall (Γ : list nat) (f6 : term) (args : list term),
+  ~ (isConstruct f6 || isFix f6 || isRel f6) ->
+  expanded Σ Γ f6 ->
+  P Γ f6 -> Forall (expanded Σ Γ) args -> Forall (P Γ) args -> P Γ (mkApps f6 args)) ->
+  (forall (Γ : list nat) (c : kername) (u : Instance.t), P Γ (tConst c u)) ->
+  (forall (Γ : list nat) (ind : inductive) (u : Instance.t), P Γ (tInd ind u)) ->
+  (forall (Γ : list nat) (ci : case_info) (type_info : predicate term)
+    (discr : term) (branches : list (branch term)),
+  expanded Σ Γ discr ->
+  P Γ discr ->
+  Forall (expanded Σ Γ) type_info.(pparams) ->
+  Forall (P Γ) type_info.(pparams) ->
   Forall
-  (fun br : branch term =>
- P (repeat 0 #|bcontext br| ++ Γ) (bbody br)) branches ->
- P Γ (tCase ci type_info discr branches)) ->
-(forall (Γ : list nat) (proj : projection) (t : term),
- expanded Σ Γ t -> P Γ t -> P Γ (tProj proj t)) ->
-(forall (Γ : list nat) (mfix : mfixpoint term) (idx : nat) 
-   (args : list term) (d : def term),
- Forall
-   (fun d0 : def term =>
-    let ctx := rev_map (fun d1 : def term => 1 + rarg d1) mfix in
-    expanded Σ (ctx ++ Γ) (dbody d0)) mfix ->
- Forall
+    (fun br : branch term =>
+    expanded_context Σ (repeat 0 #|type_info.(pparams)|)  br.(bcontext) /\
+    expanded Σ (repeat 0 #|bcontext br| ++ Γ) (bbody br)) branches ->
+    Forall
+    (fun br : branch term =>
+      ∥ All_fold (fun Δ d => ForOption (fun b => P (repeat 0 (#|Δ| + #|type_info.(pparams)|)) b) d.(decl_body)) br.(bcontext) ∥ /\
+      P (repeat 0 #|bcontext br| ++ Γ) (bbody br)) branches ->
+      P Γ (tCase ci type_info discr branches)) ->
+  (forall (Γ : list nat) (proj : projection) (t : term),
+  expanded Σ Γ t -> P Γ t -> P Γ (tProj proj t)) ->
+  (forall (Γ : list nat) (mfix : mfixpoint term) (idx : nat) 
+    (args : list term) (d : def term),
+  Forall
     (fun d0 : def term =>
-     let ctx := rev_map (fun d1 : def term => 1 + rarg d1) mfix in
-     P (ctx ++ Γ) (dbody d0)) mfix ->
- Forall (expanded Σ Γ) args -> Forall (P Γ) args ->
- args <> [] ->
- nth_error mfix idx = Some d ->
- #|args| > rarg d -> P Γ (mkApps (tFix mfix idx) args)) ->
-(forall (Γ : list nat) (mfix : mfixpoint term) (idx : nat),
- Forall (fun d : def term => expanded Σ (repeat 0 #|mfix| ++ Γ) (dbody d))
-   mfix ->  Forall (fun d : def term => P (repeat 0 #|mfix| ++ Γ) (dbody d))
-   mfix  -> P Γ (tCoFix mfix idx)) ->
-(forall (Γ : list nat) (ind : inductive) (c : nat) 
-   (u : Instance.t) (mind : mutual_inductive_body)
-   (idecl : one_inductive_body) (cdecl : constructor_body) 
-   (args : list term),
- declared_constructor Σ (ind, c) mind idecl cdecl ->
- #|args| >= ind_npars mind + context_assumptions (cstr_args cdecl) ->
- Forall (expanded Σ Γ) args -> Forall (P Γ) args -> P Γ (mkApps (tConstruct ind c u) args)) ->
-forall (Γ : list nat) (t : term), expanded Σ Γ t -> P Γ t.
+      let ctx := rev_map (fun d1 : def term => 1 + rarg d1) mfix in
+      expanded Σ (ctx ++ Γ) (dbody d0)) mfix ->
+  Forall
+      (fun d0 : def term =>
+      let ctx := rev_map (fun d1 : def term => 1 + rarg d1) mfix in
+      P (ctx ++ Γ) (dbody d0)) mfix ->
+  Forall (expanded Σ Γ) args -> Forall (P Γ) args ->
+  args <> [] ->
+  nth_error mfix idx = Some d ->
+  #|args| > rarg d -> P Γ (mkApps (tFix mfix idx) args)) ->
+  (forall (Γ : list nat) (mfix : mfixpoint term) (idx : nat),
+  Forall (fun d : def term => expanded Σ (repeat 0 #|mfix| ++ Γ) (dbody d))
+    mfix ->  Forall (fun d : def term => P (repeat 0 #|mfix| ++ Γ) (dbody d))
+    mfix  -> P Γ (tCoFix mfix idx)) ->
+  (forall (Γ : list nat) (ind : inductive) (c : nat) 
+    (u : Instance.t) (mind : mutual_inductive_body)
+    (idecl : one_inductive_body) (cdecl : constructor_body) 
+    (args : list term),
+  declared_constructor Σ (ind, c) mind idecl cdecl ->
+  #|args| >= ind_npars mind + context_assumptions (cstr_args cdecl) ->
+  Forall (expanded Σ Γ) args -> Forall (P Γ) args -> P Γ (mkApps (tConstruct ind c u) args)) ->
+  forall (Γ : list nat) (t : term), expanded Σ Γ t -> P Γ t.
 Proof.
   intros Σ P HRel HVar HEvar HSort HProd HLamdba HLetIn HApp HConst HInd HCase HProj HFix HCoFix HConstruct.
   fix f 3.
@@ -115,6 +128,13 @@ Proof.
   - eapply HEvar; eauto. clear - f H. induction H; econstructor; eauto.
   - eapply HApp; eauto. clear - f H0. induction H0; econstructor; eauto.
   - eapply HCase; eauto. induction H; econstructor; eauto.
+    clear -H1 f. induction H1; constructor; auto.
+    clear -H0 f.
+    revert H0. induction 1; constructor; auto.
+    split. destruct H as [[] ?]; constructor; auto.
+    clear -X f. induction X; constructor; auto. destruct p; constructor; auto.
+    apply f. rewrite repeat_app. exact H.
+    eapply f, H.
   - assert (Forall (P Γ) args). { clear - H0 f. induction H0; econstructor; eauto. }
     eapply HFix; eauto.
     revert H. clear - f.
@@ -124,4 +144,280 @@ Proof.
     generalize mfix at 1 3. intros mfix0 H.  induction H; econstructor; cbn in *; eauto; split.
   - eapply HConstruct; eauto.
     clear - H1 f. induction H1; econstructor; eauto.
+Qed.
+
+Record expanded_constant_decl Σ (cb : constant_body) : Prop :=
+  { expanded_body : on_Some_or_None (expanded Σ []) cb.(cst_body); }.
+    (* expanded_type : expanded Σ [] cb.(Ast.Env.cst_type) }. *)
+
+Record expanded_constructor_decl Σ mdecl cdecl :=
+  { expanded_cstr_args : expanded_context Σ (repeat 0 (#|mdecl.(ind_params)| + #|mdecl.(ind_bodies)|)) cdecl.(cstr_args) }.
+    (* expanded_cstr_indices : All (expanded Σ []) cdecl.(cstr_indices); *)
+    (* expanded_cstr_type : expanded Σ (repeat 0 #|mdecl.(ind_bodies)|) cdecl.(cstr_type) }. *)
+    
+Record expanded_inductive_decl Σ mdecl idecl :=
+  { (* expanded_ind_type : expanded Σ [] idecl.(ind_type); *)
+    expanded_ind_ctors : Forall (expanded_constructor_decl Σ mdecl) idecl.(ind_ctors) }.
+
+Record expanded_minductive_decl Σ mdecl :=
+  { expanded_params : expanded_context Σ [] mdecl.(ind_params);
+    expanded_ind_bodies : Forall (expanded_inductive_decl Σ mdecl) mdecl.(ind_bodies) }.
+
+Definition expanded_decl Σ d :=
+  match d with
+  | ConstantDecl cb => expanded_constant_decl Σ cb
+  | InductiveDecl idecl => expanded_minductive_decl Σ idecl
+  end.
+        
+Inductive expanded_global_declarations (univs : ContextSet.t) : forall (Σ : global_declarations), Prop :=
+| expanded_global_nil : expanded_global_declarations univs []
+| expanded_global_cons decl Σ : expanded_global_declarations univs Σ -> 
+  expanded_decl {| universes := univs; declarations := Σ |} decl.2 ->
+  expanded_global_declarations univs (decl :: Σ).
+
+Definition expanded_global_env (g : global_env) :=
+  expanded_global_declarations g.(universes) g.(declarations).
+
+Definition expanded_pcuic_program (p : pcuic_program) :=
+  expanded_global_env p.1 /\ expanded p.1 [] p.2.
+
+
+From Coq Require Import ssreflect.
+From Equations Require Import Equations.
+
+From MetaCoq.PCUIC Require Import PCUICInductiveInversion PCUICLiftSubst PCUICSigmaCalculus.
+
+Lemma All_tip {A} {P : A -> Type} {a : A} : P a <~> All P [a].
+Proof. split; intros. repeat constructor; auto. now depelim X. Qed.
+
+Lemma expanded_mkApps_expanded {Σ Γ f args} : 
+  expanded Σ Γ f -> All (expanded Σ Γ) args ->
+  expanded Σ Γ (mkApps f args).
+Proof.
+  intros.
+  destruct (isConstruct f || isFix f || isRel f) eqn:eqc.
+  destruct f => //.
+  - depelim H; solve_discr. eapply expanded_tRel; tea. cbn in Hle. lia. solve_all.
+    destruct args0 using rev_case; cbn in *; subst. cbn in H. congruence.
+    rewrite mkApps_app in H2; noconf H2.
+  - depelim H; solve_discr.
+    destruct args0 using rev_case; cbn in *; subst. cbn in H. congruence.
+    rewrite mkApps_app in H2; noconf H2.
+    eapply expanded_tConstruct_app; tea. cbn in H0. lia. solve_all.
+  - depelim H; solve_discr.
+    destruct args0 using rev_case; cbn in *; subst. cbn in H. congruence.
+    rewrite mkApps_app in H2; noconf H2.
+  - eapply expanded_mkApps. now rewrite eqc. auto. solve_all.
+Qed.
+
+Lemma expanded_lift Σ n k b Γ Δ Δ' : 
+  #|Γ| = k ->
+  #|Δ'| = n ->
+  expanded Σ (Γ ++ Δ) b -> 
+  expanded Σ (Γ ++ Δ' ++ Δ) (lift n k b).
+Proof.
+  intros Hk Hn.
+  remember (Γ ++ Δ)%list as Γ_.
+  intros exp; revert Γ n k Hn Hk HeqΓ_.
+  induction exp using expanded_ind; intros Γ' n' k Hn Hk ->.
+  all:try solve[ cbn; econstructor => // ].
+  2,7:try solve [cbn; econstructor => //; solve_all ].
+  - subst n'. rewrite lift_mkApps /=.
+    destruct (Nat.leb_spec k n).
+    * rewrite nth_error_app_ge in H. lia.
+      eapply expanded_tRel.
+      rewrite nth_error_app_ge; [lia|].
+      rewrite nth_error_app_ge; [lia|]. erewrite <- H. lia_f_equal.
+      now len. solve_all.
+    * eapply expanded_tRel.
+      rewrite nth_error_app_lt in H; [lia|].
+      rewrite nth_error_app_lt; [lia|]. tea. now len. solve_all.
+  - cbn. econstructor.
+    eapply (IHexp (0 :: Γ') n' (S k)); cbn; auto; lia.
+  - cbn. econstructor. apply IHexp1; auto.
+    eapply (IHexp2 (0 :: Γ') n' (S k)); cbn; auto; lia.
+  - rewrite lift_mkApps.
+    destruct (isConstruct (lift n' k f6) || isFix (lift n' k f6) || isRel (lift n' k f6)) eqn:eqc.
+    specialize (IHexp  _ _ _ Hn Hk eq_refl).
+    eapply expanded_mkApps_expanded => //. solve_all.
+    eapply expanded_mkApps => //. now rewrite eqc. now eapply IHexp. solve_all.
+  - cbn. econstructor. eauto. solve_all. cbn. solve_all.
+    solve_all.
+    specialize (H1 (repeat 0 #|bcontext x| ++ Γ') n' (#|bcontext x| + k) Hn).
+    forward H1. len.
+    forward H1. now rewrite app_assoc.
+    rewrite /id. rewrite app_assoc. apply H1.
+  - rewrite lift_mkApps. cbn.
+    eapply expanded_tFix.
+    + solve_all.
+      specialize (a 
+      (rev_map (fun d0 : def term => S (rarg d0))
+      (map (map_def (lift n' k) (lift n' (#|mfix| + k))) mfix) ++ Γ') n' (#|mfix| + k) Hn).
+      forward a. { rewrite rev_map_spec; len. }
+      forward a. { rewrite app_assoc. f_equal. f_equal.
+        rewrite !rev_map_spec. f_equal. now rewrite map_map_compose /=. }
+      rewrite app_assoc. eapply a.
+    + solve_all.
+    + destruct args => //.
+    + rewrite nth_error_map /= H4 //.
+    + len.
+  - cbn. constructor.
+    solve_all.
+    specialize (a (repeat 0 #|mfix| ++ Γ') n' (#|mfix| + k) Hn).
+    forward a. { len. }
+    forward a. { rewrite app_assoc //. }
+    rewrite app_assoc. eapply a.
+  - rewrite lift_mkApps. cbn.
+    eapply expanded_tConstruct_app; tea. now len.
+    solve_all.
+Qed.
+
+Lemma expanded_subst Σ a k b Γ Δ : 
+    #|Γ| = k ->
+  Forall (expanded Σ Δ) a -> 
+  expanded Σ (Γ ++ repeat 0 #|a| ++ Δ) b -> 
+  expanded Σ (Γ ++ Δ) (subst a k b).
+Proof.
+  intros Hk H.
+  remember (Γ ++ _ ++ Δ)%list as Γ_.
+  intros exp; revert Γ k Hk HeqΓ_.
+  induction exp using expanded_ind; intros Γ' k Hk ->.
+  all:try solve[ cbn; econstructor => // ].
+  2,7:solve[ cbn; econstructor => //; solve_all ].
+  - rewrite subst_mkApps /=.
+    destruct (Nat.leb_spec k n).
+    destruct (nth_error a _) eqn:hnth.
+    * eapply expanded_mkApps_expanded.
+      eapply nth_error_forall in H; tea.  
+      eapply (expanded_lift Σ k 0 _ [] Δ Γ'); auto.
+      solve_all. 
+    * rewrite nth_error_app_ge in H0. lia.
+      eapply nth_error_None in hnth.
+      rewrite nth_error_app_ge in H0. rewrite repeat_length. lia.
+      rewrite repeat_length in H0.
+      eapply expanded_tRel. rewrite nth_error_app_ge. lia. erewrite <- H0.
+      lia_f_equal. len. solve_all.
+    * rewrite nth_error_app_lt in H0. lia.  
+      eapply expanded_tRel. rewrite nth_error_app_lt. lia. tea. now len.
+      solve_all.
+  - cbn. econstructor.
+    eapply (IHexp (0 :: Γ') (S k)); cbn; auto; lia.
+  - cbn. econstructor. apply IHexp1; auto.
+    eapply (IHexp2 (0 :: Γ') (S k)); cbn; auto; lia.
+  - rewrite subst_mkApps.
+    destruct (isConstruct (subst a k f6) || isFix (subst a k f6) || isRel (subst a k f6)) eqn:eqc.
+    specialize (IHexp  _ _ Hk eq_refl).
+    eapply expanded_mkApps_expanded => //. solve_all.
+    eapply expanded_mkApps => //. now rewrite eqc. now eapply IHexp. solve_all.
+  - cbn. econstructor. eauto. cbn. solve_all. solve_all.
+    specialize (H2 (repeat 0 #|bcontext x| ++ Γ') (#|bcontext x| + k)).
+    forward H2 by len.
+    forward H2. now rewrite app_assoc.
+    rewrite /id. rewrite app_assoc. apply H2.
+  - rewrite subst_mkApps. cbn.
+    eapply expanded_tFix.
+    + solve_all.
+      specialize (a0 
+      (rev_map (fun d0 : def term => S (rarg d0))
+      (map (map_def (subst a k) (subst a (#|mfix| + k))) mfix) ++ Γ') (#|mfix| + k)).
+      forward a0 by len.
+      forward a0. { rewrite app_assoc. f_equal. f_equal.
+        rewrite !rev_map_spec. f_equal. now rewrite map_map_compose /=. }
+      rewrite app_assoc. eapply a0.
+    + solve_all.
+    + now destruct args.
+    + rewrite nth_error_map /= H5 //.
+    + len. 
+  - cbn. constructor.
+    solve_all.
+    specialize (a0 (repeat 0 #|mfix| ++ Γ') (#|mfix| + k)).
+    forward a0 by len.
+    forward a0. { rewrite app_assoc //. }
+    rewrite app_assoc. eapply a0.
+  - rewrite subst_mkApps. cbn.
+    eapply expanded_tConstruct_app; tea. now len.
+    solve_all.
+Qed.
+
+Lemma All_fold_tip {A : Type} (P : list A -> A -> Type) {x} : All_fold P [x] -> P [] x.
+Proof.
+  intros a; now depelim a.
+Qed.
+
+Lemma expanded_let_expansion Σ (Δ : context) Γ t :
+  expanded_context Σ Γ Δ ->
+  expanded Σ (repeat 0 #|Δ| ++ Γ) t ->
+  expanded Σ (repeat 0 (context_assumptions Δ) ++ Γ) (expand_lets Δ t).
+Proof.
+  intros [ha].
+  revert Γ t ha.
+  induction Δ using PCUICInduction.ctx_length_rev_ind.
+  - cbn; intros. now rewrite expand_lets_nil.
+  - intros Γ' t ha; destruct d as [na [b|] ty]; cbn; len; cbn.
+    * rewrite expand_lets_vdef /= //.
+      intros exp. relativize (context_assumptions Γ).
+      eapply H. now len.
+      { eapply All_fold_app_inv in ha as [].
+        depelim a. depelim a. cbn in *.
+        rewrite /subst_context.
+        eapply PCUICParallelReduction.All_fold_fold_context_k.
+        eapply All_fold_impl; tea. cbn; intros.
+        depelim f.
+        destruct decl_body => //; constructor. depelim H1.
+        len in H1. cbn in H1.
+        cbn. len. eapply expanded_subst. now rewrite repeat_length. eauto.
+        auto. cbn. now rewrite repeat_app /= -app_assoc /= in H1. }
+      len.
+      rewrite repeat_app -app_assoc /= in exp.
+      eapply All_fold_app_inv in ha as []. eapply All_fold_tip in a. cbn in a. depelim a.
+      eapply expanded_subst. rewrite repeat_length //. constructor; auto.
+      cbn. exact exp. now len.
+    * rewrite expand_lets_vass /= //.
+      rewrite !repeat_app -!app_assoc.
+      intros exp. relativize (context_assumptions Γ).
+      eapply H. lia.  
+      { eapply All_fold_app_inv in ha as [].
+        depelim a. cbn in f. depelim a.
+        eapply All_fold_impl; tea. cbn; intros.
+        destruct decl_body => //; constructor. depelim H0. len in H0. cbn in H0.
+        now rewrite repeat_app /= -app_assoc /= in H0. }
+      exact exp. lia.
+Qed.
+
+Require Import PCUICUnivSubst.
+
+Lemma subst_instance_isConstruct t u : isConstruct t@[u] = isConstruct t.
+Proof. destruct t => //. Qed.
+Lemma subst_instance_isRel t u : isRel t@[u] = isRel t.
+Proof. destruct t => //. Qed.
+Lemma subst_instance_isFix t u : isFix t@[u] = isFix t.
+Proof. destruct t => //. Qed.
+
+Lemma expanded_subst_instance Σ Γ t u : expanded Σ Γ t -> expanded Σ Γ t@[u].
+Proof.
+  induction 1 using PCUICEtaExpand.expanded_ind; cbn.
+  all:intros; rewrite ?subst_instance_mkApps.
+  all:try solve [econstructor; eauto 1].
+  - econstructor; eauto. now rewrite map_length. solve_all.
+  - econstructor; eauto. solve_all.
+  - econstructor; eauto. 2:solve_all.
+    rewrite subst_instance_isConstruct subst_instance_isFix subst_instance_isRel //.
+  - econstructor; eauto. cbn. solve_all.
+    solve_all. 
+  - cbn; eapply expanded_tFix. solve_all. 
+    rewrite rev_map_spec map_map_compose -rev_map_spec //.
+    solve_all. now destruct args => //.
+    rewrite nth_error_map H4 //.
+    now len.
+  - econstructor; eauto. solve_all.
+  - eapply expanded_tConstruct_app; tea. now len. solve_all.
+Qed.
+
+Lemma expanded_weakening Σ Γ t : expanded Σ Γ t -> forall Γ', expanded Σ (Γ ++ Γ') t.
+Proof.
+  induction 1 using PCUICEtaExpand.expanded_ind; cbn.
+  1:{ intros. eapply expanded_tRel; tea. rewrite nth_error_app_lt.
+     now eapply nth_error_Some_length in H. assumption.
+    solve_all. }
+  all:intros; try solve [econstructor; eauto 1; solve_all; try now rewrite app_assoc].
 Qed.
