erasure/theories/EProgram.v
@@ -1,0 +1,106 @@
+(* Distributed under the terms of the MIT license. *)
+From Coq Require Import Program ssreflect ssrbool.
+From Equations Require Import Equations.
+From MetaCoq.Template Require Import Transform bytestring config utils BasicAst.
+From MetaCoq.PCUIC Require PCUICAst PCUICAstUtils PCUICProgram.
+From MetaCoq.SafeChecker Require Import PCUICErrors PCUICWfEnvImpl.
+From MetaCoq.Erasure Require EAstUtils ErasureFunction ErasureCorrectness EPretty Extract.
+From MetaCoq.Erasure Require ErasureFunction EOptimizePropDiscr ERemoveParams EWcbvEval EDeps.
+
+Import bytestring.
+Local Open Scope bs.
+Local Open Scope string_scope2.
+
+Import Transform.
+
+Obligation Tactic := program_simpl.
+
+Import PCUICProgram.
+
+Definition build_wf_env_from_env {cf : checker_flags} (Σ : global_env_map) (wfΣ : ∥ PCUICTyping.wf Σ ∥) : wf_env := 
+  {| wf_env_referenced := {| referenced_impl_env := Σ.(trans_env_env); referenced_impl_wf := wfΣ |} ;
+     wf_env_map := Σ.(trans_env_map);
+     wf_env_map_repr := Σ.(trans_env_repr);
+ |}.
+
+Import EGlobalEnv.
+
+Definition eprogram := (EAst.global_context * EAst.term).
+
+Import EEnvMap.GlobalContextMap (make, global_decls).
+
+Arguments EWcbvEval.eval {wfl} _ _ _.
+
+Definition closed_eprogram (p : eprogram) := 
+  closed_env p.1 && ELiftSubst.closedn 0 p.2.
+
+Definition eval_eprogram (wfl : EWcbvEval.WcbvFlags) (p : eprogram) (t : EAst.term) := 
+  ∥ EWcbvEval.eval (wfl:=wfl) p.1 p.2 t ∥.
+
+Definition eprogram_env := 
+  (EEnvMap.GlobalContextMap.t * EAst.term).
+
+Definition closed_eprogram_env (p : eprogram_env) := 
+  let Σ := p.1.(global_decls) in
+  closed_env Σ && ELiftSubst.closedn 0 p.2.
+
+Definition eval_eprogram_env (wfl : EWcbvEval.WcbvFlags) (p : eprogram_env) (t : EAst.term) := 
+  ∥ EWcbvEval.eval (wfl:=wfl) p.1.(global_decls) p.2 t ∥.
+
+Lemma wf_glob_fresh Σ : wf_glob Σ -> EnvMap.EnvMap.fresh_globals Σ.
+Proof.
+  induction Σ. constructor; auto.
+  intros wf; depelim wf. constructor; auto.
+Qed.
+  
+Program Definition erase_pcuic_program (p : pcuic_program) 
+  (wfΣ : ∥ PCUICTyping.wf_ext (H := config.extraction_checker_flags) p.1 ∥)
+  (wt : ∥ ∑ T, PCUICTyping.typing (H := config.extraction_checker_flags) p.1 [] p.2 T ∥) : eprogram_env :=
+  let wfe := build_wf_env_from_env p.1.1 (map_squash (PCUICTyping.wf_ext_wf _) wfΣ) in
+  let wfe' := ErasureFunction.make_wf_env_ext wfe p.1.2 wfΣ in
+  let t := ErasureFunction.erase wfe' nil p.2 _ in
+  let Σ' := ErasureFunction.erase_global (EAstUtils.term_global_deps t) wfe in
+  (EEnvMap.GlobalContextMap.make Σ' _, t).
+  
+Next Obligation.
+  sq. destruct wt as [T Ht].
+  cbn in *. subst. now exists T.
+Qed.
+Next Obligation.
+  unfold ErasureFunction.erase_global.
+  eapply wf_glob_fresh.
+  eapply ErasureFunction.erase_global_decls_wf_glob.
+Qed.
+
+Obligation Tactic := idtac.
+
+Import Extract.
+
+Definition expanded_eprogram (p : eprogram_env) := 
+  let decls := p.1.(EEnvMap.GlobalContextMap.global_decls) in
+  EEtaExpandedFix.isEtaExp_env decls && EEtaExpandedFix.isEtaExp decls [] p.2.
+
+Definition expanded_eprogram_cstrs (p : eprogram_env) := 
+  let decls := p.1.(EEnvMap.GlobalContextMap.global_decls) in
+  EEtaExpanded.isEtaExp_env decls && EEtaExpanded.isEtaExp decls p.2.
+  
+Definition erase_program (p : pcuic_program) (wtp : ∥ wt_pcuic_program (cf:=config.extraction_checker_flags) p ∥) : eprogram_env :=
+  erase_pcuic_program p (map_squash fst wtp) (map_squash snd wtp).
+
+Lemma expanded_erase_program (cf := config.extraction_checker_flags) p (wtp : ∥ wt_pcuic_program p ∥) :
+  PCUICEtaExpand.expanded_pcuic_program p ->
+  expanded_eprogram (erase_program p wtp).
+Proof.
+  intros [etaenv etat]. apply /andP; split.
+  eapply EEtaExpandedFix.expanded_global_env_isEtaExp_env, ErasureFunction.expanded_erase_global, etaenv.
+  eapply EEtaExpandedFix.expanded_isEtaExp, ErasureFunction.expanded_erase, etat.
+Qed.
+
+Lemma expanded_eprogram_expanded_eprogram_cstrs p :
+  expanded_eprogram p ->
+  expanded_eprogram_cstrs p.
+Proof.
+  move=> /andP[] etaenv etat.
+  apply /andP. split; [now eapply EEtaExpanded.isEtaExpFix_env_isEtaExp_env|
+  now eapply EEtaExpanded.isEtaExpFix_isEtaExp].
+Qed.
