pcuic/theories/PCUICTransform.v
@@ -1,0 +1,94 @@
+(** * Definition of programs in template-coq, well-typed terms and provided transformations **)
+From Coq Require Import ssreflect.
+From MetaCoq.Template Require Import utils config Transform.        
+From MetaCoq.Template Require TemplateProgram.
+Import TemplateProgram (template_program, wt_template_program, eval_template_program).
+
+From MetaCoq.PCUIC Require Import PCUICAstUtils PCUICAst TemplateToPCUIC
+    PCUICGlobalEnv PCUICTyping PCUICEtaExpand
+    PCUICProgram.
+From MetaCoq.PCUIC Require TemplateToPCUICWcbvEval
+  TemplateToPCUICCorrectness 
+  TemplateToPCUICExpanded.
+    
+Import Transform.
+
+(** * Translation from Template to PCUIC, directly preserves evaluation *)
+
+Definition eval_pcuic_program (p : pcuic_program) (v : term) :=
+  ∥ PCUICWcbvEval.eval p.1.(trans_env_env) p.2 v ∥.
+      
+Definition template_to_pcuic_obseq (p : template_program) (p' : pcuic_program) (v : Ast.term) (v' : term) :=
+  let Σ := Ast.Env.empty_ext p.1 in v' = trans (trans_global Σ) v.
+
+Lemma trans_template_program_wt {cf : checker_flags} p (wtp : wt_template_program p) : wt_pcuic_program (trans_template_program p).
+Proof.
+  move: p wtp.
+  intros [Σ t] [wfext ht].
+  unfold wt_pcuic_program, trans_template_program; cbn in *.
+  cbn. split. eapply TemplateToPCUICCorrectness.template_to_pcuic_env_ext in wfext. apply wfext.
+  destruct ht as [T HT]. exists (trans (trans_global_env Σ) T).
+  eapply (TemplateToPCUICCorrectness.template_to_pcuic_typing (Σ := Ast.Env.empty_ext Σ) []). apply wfext.
+  apply HT.
+Qed.
+
+Local Obligation Tactic := idtac.
+
+Program Definition template_to_pcuic_transform {cf : checker_flags} : 
+  Transform.t template_program pcuic_program Ast.term term 
+  eval_template_program eval_pcuic_program :=
+ {| name := "template to pcuic";
+    pre p := ∥ wt_template_program p ∥ /\ EtaExpand.expanded_program p ;
+    transform p _ := trans_template_program p ;
+    post p := ∥ wt_pcuic_program p ∥ /\ PCUICEtaExpand.expanded_pcuic_program p;
+    obseq := template_to_pcuic_obseq |}.
+Next Obligation.
+  cbn. intros cf p [[wtp] etap].
+  split; [split|].
+  now eapply trans_template_program_wt.
+  now eapply TemplateToPCUICExpanded.expanded_trans_program in etap.
+Qed.
+Next Obligation.
+  red. intros cf [Σ t] v [[]].
+  unfold eval_pcuic_program, eval_template_program.
+  cbn. intros [ev].
+  unshelve eapply TemplateToPCUICWcbvEval.trans_wcbvEval in ev; eauto. apply X.
+  eexists; split; split; eauto.
+  eapply TemplateToPCUICCorrectness.template_to_pcuic_env.
+  apply X. destruct X as [wfΣ [T HT]]. apply TypingWf.typing_wf in HT. apply HT. auto.
+Qed.
+
+From MetaCoq.PCUIC Require Import PCUICExpandLets PCUICExpandLetsCorrectness.
+
+(** Expansion of let bindings in constructor types / case branches. 
+    Direcly preserves evaluation as well: the new value is simply the 
+    expansion of the old one, which is the identiy on normal forms.
+*)
+
+Definition let_expansion_obseq (p : pcuic_program) (p' : pcuic_program) (v : term) (v' : term) :=
+  v' = PCUICExpandLets.trans v.
+
+Program Definition pcuic_expand_lets_transform {cf : checker_flags} : 
+  self_transform pcuic_program term eval_pcuic_program eval_pcuic_program :=
+ {| name := "let expansion in branches/constructors";
+    pre p := ∥ wt_pcuic_program p ∥ /\ PCUICEtaExpand.expanded_pcuic_program p ;
+    transform p hp := expand_lets_program p;
+    post p := ∥ wt_pcuic_program (cf:=PCUICExpandLetsCorrectness.cf' cf) p ∥ /\ PCUICEtaExpand.expanded_pcuic_program p;
+    obseq := let_expansion_obseq |}.
+Next Obligation.
+  intros cf [Σ t] [[[wfext ht]] etap].
+  cbn. split. sq. unfold build_global_env_map. unfold global_env_ext_map_global_env_ext. simpl.
+  split. eapply PCUICExpandLetsCorrectness.trans_wf_ext in wfext. apply wfext.
+  destruct ht as [T HT]. exists (PCUICExpandLets.trans T).
+  eapply (PCUICExpandLetsCorrectness.pcuic_expand_lets Σ []) => //.
+  apply wfext. apply PCUICExpandLetsCorrectness.trans_wf_ext in wfext. apply wfext.
+  now eapply expanded_expand_lets_program.
+Qed.
+Next Obligation.
+  red. intros cf [Σ t] v [[]].
+  unfold eval_pcuic_program.
+  cbn. intros [ev]. destruct X.
+  eapply (PCUICExpandLetsCorrectness.trans_wcbveval (Σ:=global_env_ext_map_global_env_ext Σ)) in ev.
+  eexists; split; split; eauto.
+  destruct s as [T HT]. now apply PCUICClosedTyp.subject_closed in HT.
+Qed.
